\section{Attempts at relativistic quantum mechanics}

\begin{equation}
	i\hbar \pdfrac{}{t}\ket{\psi, t} = H \ket{\psi, t}.
\end{equation}

\begin{equation}
	H = \frac{1}{2m} \mathbf{P}^2.
\end{equation}

\begin{equation}
	i\hbar \pdfrac{}{t}\psi(\mathbf{x}, t)= -\frac{\hbar^2}{2m} \nabla^2 \psi(\mathbf{x}, t).
\end{equation}

\begin{equation}
	H = + \sqrt{\mathbf{P}^2 c^2 + m^2 c^4}.
\end{equation}

\begin{equation}
	H = mc^2 + \frac{1}{2m}\mathbf{P}^2 + \cdots.
\end{equation}

\begin{equation}
	i\hbar \pdfrac{}{t} \psi(\mathbf{x}, t) = + \sqrt{- \hbar^2 c^2 \nabla^2 + m^2 c^4}\ \psi(\mathbf{x}, t).
\end{equation}

\begin{equation}
	- \hbar^2 \pdfrac{{}^2}{t^2} \psi(\mathbf{x}, t) = \left( - \hbar^2 c^2 \nabla^2 + m^2 c^4 \right) \ \psi(\mathbf{x}, t)	.
\end{equation}

\begin{equation}
	g_{\mu\nu} = 
	\begin{pmatrix}
		-1 & & & \\
		& 1 & & \\
		& & 1 & \\
		& & & 1
	\end{pmatrix}.
\end{equation}

\begin{equation}
	g^{\mu\nu} = 
	\begin{pmatrix}
		-1 & & & \\
		& 1 & & \\
		& & 1 & \\
		& & & 1
	\end{pmatrix}.
\end{equation}

\begin{equation}
	\bar{x}^\mu = \Lambda^{\mu}{}_\nu x^\nu + a^\mu.
\end{equation}

\begin{equation}
	g_{\mu\nu} \Lambda^\mu{}_\rho \Lambda^{\nu}{}_\sigma = g_{\rho\sigma}.
\end{equation}

\begin{equation}\begin{aligned}
	(x - x^\prime)^2 & \equiv g_{\mu\nu} (x - x^\prime)^\mu (x - x^\prime)^\nu \\
	& = (\mathbf{x} - \mathbf{x}^\prime)^2 - c^2 (t - t^\prime)^2.
\end{aligned}\end{equation}

\begin{equation}\begin{aligned}
	(\bar{x} - \bar{x}^\prime)^2 & = g_{\mu\nu} (\bar{x} - \bar{x}^\prime)^\mu (\bar{x} - \bar{x}^\prime)^\nu \\
	& = g_{\mu\nu} \Lambda^\mu{}_\rho \Lambda^\nu{}_\sigma (x - x^\prime)^\rho (x - x^\prime)^\sigma \\ 
	& = g_{\rho\sigma} (x - x^\prime)^\rho (x - x^\prime)^\sigma \\ 
	& = (x - x^\prime)^2.
\end{aligned}\end{equation}

\begin{align}
	& \partial_\mu \equiv \pdfrac{}{x^\mu} = \left( + \frac{1}{c} \pdfrac{}{t}, \nabla \right), \\
	& \partial^\mu \equiv \pdfrac{}{x_\mu} = \left( - \frac{1}{c} \pdfrac{}{t}, \nabla \right).
\end{align}

\begin{equation}
	\partial^\mu x^\nu = g^{\mu\nu}.
\end{equation}

\begin{equation}
	\bar\partial^\mu = \Lambda^\mu{}_\nu \partial^\nu.
\end{equation}

\begin{equation}
	\bar\partial^\rho \bar{x}^\sigma = (\Lambda^\rho{}_\mu \partial^\mu)(\Lambda^\sigma{}_\nu x^\nu + a^\sigma) = \Lambda^\rho{}_\mu \Lambda^\sigma{}_\nu (\partial^\mu x^\nu) = \Lambda^\rho{}_\mu \Lambda_\sigma{}_\nu g^{\mu\nu} = g^{\rho\sigma}.
\end{equation}

\begin{equation}
	- \hbar^2 c^2 \partial_0^2 \psi(x) = (- \hbar^2 c^2 \nabla^2 + m^2 c^4) \psi(x).
\end{equation}

\begin{equation}
	(- \partial^2 + m^2 c^2 / \hbar^2) \psi(x) = 0.
\end{equation}

\begin{equation}
	(- \bar\partial^2 + m^2 c^2 / \hbar^2) \bar\psi(\bar{x}) = 0.
\end{equation}

\begin{equation}
	\bar\partial^2 = g_{\mu\nu} \bar\partial^\mu \bar\partial^\nu = g_{\mu\nu} \Lambda^\mu{}_\rho \Lambda^\nu{}_\sigma \partial^\rho \partial^\sigma = \partial^2.
\end{equation}

\begin{equation}
	\braket{\psi, t}{\psi ,t} = \int \dd{3}{x} \braket{\psi, t}{\mathbf{x}} \braket{\mathbf{x}}{\psi, t} = \int \dd{3}{x} \psi^*(x) \psi(x).
\end{equation}

\begin{equation}
	i\hbar \pdfrac{}{t} \psi_a(x) = \left( -i\hbar c \left(\alpha^j\right)_{ab} \partial_j + mc^2 (\beta)_{ab} \right) \psi_b (x).
\end{equation}

\begin{equation}
	H_{ab} = c P_j \left( \alpha^j \right)_{ab} + mc^2 (\beta)_{ab}.
\end{equation}